\documentclass{article} 
\begin{document}
prove that 
\( \displaystyle \sum_{ 0 \le i \le n }  x _{i} ^{k} l _{i} (x) = x ^{k}\)

It is known that \( \displaystyle \sum_{   0 \le i \le n }   l _{i} (x)  =  1\)

For that the function \( \displaystyle  F (x)  = \sum_{   0  \le i \le n }  l _{i}  (x)  -  1\) is polynomial and 
have \(n + 1 \) roots. 

So the function must be a constant. 



We need to prove that 
\[
	\sum_{ 0 \le i \le n} x _{i} ^{k} l_{i} (x) = x ^{k} 
\]
that is prove that 
\[
	\left(\sum _{0 \le i \le n } x _{i} ^{k }  l _{i} (x)  \right) \Big/ x ^{k} = 1 
\]
Similarily, 
\[
	F (x) = \left( \sum _{0 \le i \le n}  x _{i} ^{k} l _{i} (x) \right)\!\! \Bigg/\, x ^{k}   - 1 
\]
have \(  n  + 1\) roots thus that  \(F (x) \) is a constant. 
\end{document}
